## 5.1.3
Let P(n) be the statement P(n): 1^2 + 2^2 + ... + n^2 = n(n+1)(2n+1)/6

a) What is the statement P(1)?
P(1): 1^2 = 1(1+1)(2(1) + 1)/6

b) Show that P(1) is true, completing the base step of the proof.

1) 1^2 = 6/6 ...

c) What is the inductive hypothesis?

Let k be an arbitrary positive integer.
Let P(k) be: 1^2 + 2^2 + ... + k^2 = k(k+1)(2k+1)/6

d) Prove that P(k + 1) is true based on the assumption that P(k) is true for arbitrary positive integer k where P(k + 1) is

  P(k + 1) = 1^2 + 2^2 + ... + k^2 + (k + 1)^2 = (k + 1)((k + 1) + 1)(2(k + 1) + 1)/6

e) Complete the inductive step identifying where you use the I.H.

  Proof: that P(k + 1) is true

  1^2 + 2^2 + ... + k^2 + (k + 1)^2 = k(k+1)(2k+1)/6 + (k+1)^2 (I.H.)
                                    = (k + 1)[ (k+(2k+1) + 6(k + 1))/6 ]
                                    = (k+1)/6 * (2k^2 + k + 6k + 6)
                                    = (k+1)/6 [2k^2 + 7k + 6]
                                    = (k+1)/6 (k+2)(2k+3)
                                    = (k+1)((k+1) + 1)(2(k+1) + 1)/6

                                       Hence k + 1 is true
## PMI

We have shown that P(1) is true and \ForAll k P(k) -> P(k + 1) is true, where k is an arbitrary pos. int. Hence by the PMI \ForAll n P(n) is true.
